Define the sequence $(a_n)_{n \geq 0}$ of rational numbers by $a_0 = -1$ and, for $n \geq 1$,
\[ a_n = -\sum_{k = 0}^{n - 1} \frac{a_k}{n + 1 - k}. \tag{*}\label{2006a2-eq0} \]
Prove that $a_n > 0$ for all $n \neq 0$.



\subsection*{Solution}

Official solution: \url{https://www.imo-official.org/problems/IMO2006SL.pdf}

We just present the official solution here.

The proof goes by induction on $n$, with $a_1 = 1/2 > 0$.
For induction step, suppose that $a_1, a_2, \ldots, a_n > 0$.
Note that~\eqref{2006a2-eq0} for $n > 0$ can be rewritten as
\[ \sum_{k = 0}^n \frac{a_k}{n + 1 - k} = 0. \]
The main formula for the induction step is the following: for any $n > 0$,
\begin{align*}
    (n + 2) a_{n + 1}
    &= -\sum_{k = 0}^n \frac{(n + 2) a_k}{n + 2 - k} \\
    &= \sum_{k = 0}^n \frac{(n + 1) a_k}{n + 1 - k} - \sum_{k = 0}^n \frac{(n + 2) a_k}{n + 2 - k} \\
    &= \sum_{k = 0}^n \left(\frac{n + 1}{n + 1 - k} - \frac{n + 2}{n + 2 - k}\right) a_k \\
    &= \sum_{k = 0}^n \frac{k}{(n + 1 - k)(n + 2 - k)} a_k.
\end{align*}
The term at $k = 0$ is $0$.
Since $a_1, a_2, \ldots, a_n > 0$, this gives us $(n + 2) a_{n + 1} > 0$ and thus $a_{n + 1} > 0$.
Induction step is complete.
